---
aliases: [""]
tags: ["Question","QFormat3"]
---

#### 
## Phasor manipulation

> ### $$ (a \angle \alpha) \times (b \angle \beta) = ab \angle (\alpha + \beta) $$
> ### $$ \frac{a \angle \alpha}{b \angle \beta} = \frac{a}{b} \angle (\alpha - \beta) $$ 
> ### $$ \frac{1}{a \angle \alpha} = \frac{1}{a} \angle (-\alpha) $$ 
> ### $$ (a \angle \alpha) + (b \angle \beta) = \sqrt{ a^{2} + b^{2} + 2ab \cos(\alpha - \beta) } \angle \left(\frac{\alpha+\beta}{2}\right) $$
>> where:
>> $a,b=$ [[phasor representation|phasor]] magnitudes
>> $\alpha,\beta=$ [[phasor representation|phasor]] angles
