---
aliases: [""]
tags: []
---

## Deflection of a asymmetric cross section beam


Well if you take the equations from [[bending a beam with assymetric cross sections|bending a beam with asymmetric cross sections]] and rearrange em a bit you can get:

> ### $$\begin{align*} \frac{1}{R_{yy}} &= \frac{M_{zz} I_{yy} - M_{yy} I_{yz} }{E(I_{yy} I_{zz} - I_{yz}^{2} )} = - \frac{d^{2} v}{dx^{2}} &\frac{1}{R_{zz}} &= \frac{M_{yy} I_{zz} - M_{zz} I_{yz} }{E(I_{yy} I_{zz} - I_{yz}^{2} )} = - \frac{d^{2} w}{dx^{2}}  \end{align*}$$
>> where:
>> $M_{zz},M_{yy}=$ bending moments acting in xz and xy planes respectively
>> $I_{yy}, I_{zz}=$ [[second moment of area|2nd moment of area]] (may need to use [[parallel axis theorem]])
>> $I_{yz}=$ second moment of area along yz?
>> $\sigma_{xx}=$ axial stress at some point on the beam cross section
>> $R_{y},R_{z}=$ [[Deflection in beams notes|radius of beam delfection]] in yx and zx planes respectively
>> $E=$ youngs modulus of material
>> $v=$ deflection in the y axis
>> $v=$ deflection in the z axis

^4a88d2

